work on renaming

src/coq/Renaming.v
@@ -11,26 +11,36 @@
 Require Import Ascii Strings.String.
 Require Import Vellvm.Classes Vellvm.Util.
 Require Import Vellvm.LLVMAst Vellvm.AstLib Vellvm.CFG.
+Require Import Vellvm.Memory.
 
 Open Scope string_scope.
 
 Class Swap (A:Type) := swap : raw_id -> raw_id -> A -> A.
-Class SwapLaws (A:Type) `{Swap A} := {
-  swap_same_id : forall (i:raw_id) (x:A),
-    swap i i x = x
-}.
-
 Definition swap_raw_id (id1 id2:raw_id) (id:raw_id) : raw_id :=
   if id == id1 then id2 else
     if id == id2 then id1 else
       id.
 Instance raw_id_swap : Swap raw_id := swap_raw_id.
 
+
+Class SwapLaws (A:Type) `{Swap A} := {
+  swap_same_id :
+    forall (id:raw_id) (x:A), swap id id x = x;
+
+  swap_comm:
+    forall id1 id2 (x:A), swap id1 id2 x = swap id2 id1 x;
+}.
+
 Program Instance raw_id_swaplaws : SwapLaws raw_id.
 Next Obligation.
   unfold swap. unfold raw_id_swap. unfold swap_raw_id.
-  destruct (x == i); auto.
+  destruct (x == id); auto.
 Qed.
+Next Obligation.
+  unfold swap. unfold raw_id_swap. unfold swap_raw_id.
+  destruct (x == id1); auto.
+  destruct (x == id2); auto. subst. reflexivity.
+Qed.  
 
 Definition swap_ident (id1 id2:raw_id) (id:ident) : ident :=
   match id with
@@ -47,9 +57,29 @@ Qed.
 
 Instance swap_of_pair {A B} `(SA:Swap A) `(SB:Swap B) : Swap (A * B)%type :=
   fun id1 id2 p => (swap id1 id2 (fst p), swap id2 id2 (snd p)).
-  
+
+Program Instance swap_laws_pair {A B} `(SA:Swap A) `(SB:Swap B) `(SLA:SwapLaws A) `(SLB:SwapLaws B) : SwapLaws (A*B)%type.
+Next Obligation.
+  destruct x. unfold swap. simpl. rewrite swap_comm. reflexivity.
+  unfold swap. simpl. rewrite swap_comm. reflexivity.
+Qed.
+
+
 Instance swap_of_option {A} `(SA:Swap A) : Swap (option A) :=
   fun id1 id2 opt => match opt with None => None | Some x => Some (swap id1 id2 x) end.
+
+Instance swap_of_list {A} `(SA:Swap A) : Swap (list A) :=
+  fun id1 id2 l => List.map (swap id1 id2) l.
+
+Instance swap_of_bool : Swap bool :=
+  fun id1 id2 b => b.
+
+Instance swap_of_nat : Swap nat :=
+  fun id1 id2 n => n.
+
+Instance swap_of_int : Swap int :=
+  fun id1 id2 n => n.
+
 
 Fixpoint swap_typ (id1 id2:raw_id) (t:typ) : typ :=
   match t with
@@ -137,14 +167,14 @@ Instance swap_of_instr_id : Swap instr_id := swap_instr_id.
 
 Definition swap_phi (id1 id2:raw_id) (p:phi) : phi :=
   match p with
-  | Phi t args => Phi (swap id1 id2 t) (List.map (swap id1 id2) args)
+  | Phi t args => Phi (swap id1 id2 t) (swap id1 id2 args)
   end.
 Instance swap_of_phi : Swap phi := swap_phi.
 
 Definition swap_instr (id1 id2:raw_id) (ins:instr) : instr :=
   match ins with
   | INSTR_Op op => INSTR_Op (swap id1 id2 op)
-  | INSTR_Call fn args => INSTR_Call (swap id1 id2 fn) (List.map (swap id1 id2) args)
+  | INSTR_Call fn args => INSTR_Call (swap id1 id2 fn) (swap id1 id2 args)
   | INSTR_Alloca t nb align =>
     INSTR_Alloca (swap id1 id2 t) (swap id1 id2 nb) align
   | INSTR_Load volatile t ptr align =>
@@ -160,30 +190,229 @@ Definition swap_instr (id1 id2:raw_id) (ins:instr) : instr :=
   end.
 Instance swap_of_instr : Swap instr := swap_instr.
 
-Definition mangle_instr (i:instr_id * instr) : (instr_id * instr) :=
-  match i with
-  | _ => i
+Definition swap_terminator (id1 id2:raw_id) (trm:terminator) : terminator :=
+  match trm with
+  | TERM_Ret  v => TERM_Ret (swap id1 id2 v)
+  | TERM_Ret_void => TERM_Ret_void
+  | TERM_Br v br1 br2 => TERM_Br (swap id1 id2 v) (swap id1 id2 br1) (swap id1 id2 br2)
+  | TERM_Br_1 br => TERM_Br_1 (swap id1 id2 br)
+  | TERM_Switch  v default_dest brs =>
+    TERM_Switch (swap id1 id2 v) (swap id1 id2 default_dest) (swap id1 id2 brs)
+  | TERM_IndirectBr v brs =>
+    TERM_IndirectBr (swap id1 id2 v) (swap id1 id2 brs)
+  | TERM_Resume v => TERM_Resume (swap id1 id2 v)
+  | TERM_Invoke fnptrval args to_label unwind_label =>
+    TERM_Invoke (swap id1 id2 fnptrval) (swap id1 id2 args) (swap id1 id2 to_label) (swap id1 id2 unwind_label)
   end.
+Instance swap_of_terminator : Swap terminator := swap_terminator.
 
-Definition mangle_block (blk:block) : block :=
-  blk.
+Instance swap_of_param_attr : Swap param_attr :=
+  fun id1 id2 l => l.
+Instance swap_of_fn_attr : Swap fn_attr :=
+  fun id1 id2 l => l.
 
-Definition mangle_blocks (blks:list block) : list block :=
-  List.map mangle_block blks.
+Instance swap_of_cconv : Swap cconv :=
+  fun id1 id2 l => l.
 
-Definition mangle_definition (d:definition (list block)) : definition (list block) :=
+Instance swap_of_linkage : Swap linkage :=
+  fun id1 id2 l => l.
+Instance swap_of_visibility : Swap visibility :=
+    fun id1 id2 l => l.
+Instance swap_of_dll_storage : Swap dll_storage :=
+    fun id1 id2 l => l.
+Instance swap_of_thread_local_storage : Swap thread_local_storage :=
+  fun id1 id2 l => l.
+Instance swap_of_string : Swap string :=
+  fun id1 id2 s => s.
+
+Definition swap_global (id1 id2:raw_id) (g:global) : global :=
+  mk_global 
+      (swap id1 id2 (g_ident g))
+      (swap id1 id2 (g_typ g))     
+      (swap id1 id2 (g_constant g))
+      (swap id1 id2 (g_exp g))
+      (swap id1 id2 (g_linkage g))
+      (swap id1 id2 (g_visibility g))
+      (swap id1 id2 (g_dll_storage g))
+      (swap id1 id2 (g_thread_local g))
+      (swap id1 id2 (g_unnamed_addr g))
+      (swap id1 id2 (g_addrspace g))
+      (swap id1 id2 (g_externally_initialized g))
+      (swap id1 id2 (g_section g))
+      (swap id1 id2 (g_align g)).
+
+Instance swap_of_global : Swap global := swap_global.
+
+Definition swap_declaration (id1 id2:raw_id) (d:declaration) : declaration :=
+  mk_declaration
+    (swap id1 id2 (dc_name d))
+    (swap id1 id2 (dc_type d))
+    (swap id1 id2 (dc_param_attrs d))
+    (swap id1 id2 (dc_linkage d))
+    (swap id1 id2 (dc_visibility d))
+    (swap id1 id2 (dc_dll_storage d))
+    (swap id1 id2 (dc_cconv d))
+    (swap id1 id2 (dc_attrs d))
+    (swap id1 id2 (dc_section d))
+    (swap id1 id2 (dc_align d))
+    (swap id1 id2 (dc_gc d)).
+Instance swap_of_declaration : Swap declaration := swap_declaration.    
+
+Definition swap_block (id1 id2:raw_id) (b:block) : block :=
+  mk_block (swap id1 id2 (blk_id b))
+           (swap id1 id2 (blk_phis b))
+           (swap id1 id2 (blk_code b))
+           (swap id1 id2 (blk_term b)).
+  
+Instance swap_of_block : Swap block := swap_block.
+
+Definition swap_definition {FnBody:Set} `{SF: Swap FnBody} (id1 id2:raw_id) (d:definition FnBody) : definition FnBody :=
   mk_definition _
-  (df_prototype d)
-  (df_args d)
-  (mangle_blocks (df_instrs d))
-.
+    (swap id1 id2 (df_prototype d))
+    (swap id1 id2 (df_args d))
+    (swap id1 id2 (df_instrs d)).
+
+Instance swap_of_definition {FnBody:Set} `{SF:Swap FnBody} : Swap (definition FnBody) :=
+  swap_definition.
+
+Fixpoint swap_metadata (id1 id2:raw_id) (m:metadata) : metadata :=
+  match m with
+  | METADATA_Const  tv => METADATA_Const (swap id1 id2 tv)
+  | METADATA_Null => METADATA_Null
+  | METADATA_Id id => METADATA_Id (swap id1 id2 id)
+  | METADATA_String str => METADATA_String (swap id1 id2 str)
+  | METADATA_Named strs => METADATA_Named (swap id1 id2 strs)
+  | METADATA_Node mds => METADATA_Node (List.map (swap_metadata id1 id2) mds)
+  end.
+Instance swap_of_metadata : Swap metadata := swap_metadata.
 
 
-Definition mangle_toplevel_entity (tle : toplevel_entity (list block)) : toplevel_entity (list block) :=
+Definition swap_toplevel_entity {FnBody:Set} `{SF:Swap FnBody} (id1 id2:raw_id) (tle:toplevel_entity FnBody) :=
   match tle with
-  | TLE_Definition d => TLE_Definition (mangle_definition d)
-  | _ => tle
+  | TLE_Target tgt => TLE_Target (swap id1 id2 tgt)
+  | TLE_Datalayout layout => TLE_Datalayout (swap id1 id2 layout)
+  | TLE_Declaration decl => TLE_Declaration (swap id1 id2 decl)
+  | TLE_Definition defn => TLE_Definition (swap id1 id2 defn)
+  | TLE_Type_decl id t => TLE_Type_decl (swap id1 id2 id) (swap id1 id2 t)
+  | TLE_Source_filename s => TLE_Source_filename (swap id1 id2 s)
+  | TLE_Global g => TLE_Global (swap id1 id2 g)
+  | TLE_Metadata id md => TLE_Metadata (swap id1 id2 id) (swap id1 id2 md)
+  | TLE_Attribute_group i attrs => TLE_Attribute_group (swap id1 id2 i) (swap id1 id2 attrs)
   end.
 
-Definition transform (prog: list (toplevel_entity (list block))) : list (toplevel_entity (list block)) :=
-  List.map mangle_toplevel_entity prog.
+Instance swap_of_tle {FnBody:Set} `{SF:Swap FnBody} : Swap (toplevel_entity FnBody) :=
+  swap_toplevel_entity.
+
+Definition swap_modul {FnBody:Set} `{SF:Swap FnBody} (id1 id2:raw_id) (m:modul FnBody) : modul FnBody :=
+  mk_modul _
+    (swap id1 id2 (m_name m))
+    (swap id1 id2 (m_target m))
+    (swap id1 id2 (m_datalayout m))
+    (swap id1 id2 (m_type_defs m))
+    (swap id1 id2 (m_globals m))
+    (swap id1 id2 (m_declarations m))
+    (swap id1 id2 (m_definitions m)).
+
+Instance swap_of_modul {FnBody:Set} `{SF:Swap FnBody} : Swap (modul FnBody) :=
+  swap_modul.
+
+Definition swap_pc (id1 id2:raw_id) (p:pc) : pc :=
+  mk_pc (swap id1 id2 (fn p)) (swap id1 id2 (bk p)) (swap id1 id2 (pt p)).
+
+Instance swap_of_pc : Swap pc := swap_pc.
+
+Definition swap_cmd (id1 id2:raw_id) (c:cmd) : cmd :=
+  match c with
+  | Inst i => Inst (swap id1 id2 i)
+  | Term t => Term (swap id1 id2 t)
+  end.                    
+
+Instance swap_of_cmd : Swap cmd := swap_cmd.
+
+Definition swap_cfg (id1 id2:raw_id) (CFG:cfg) : cfg :=
+  mkCFG (swap id1 id2 (init CFG)) (swap id1 id2 (blks CFG)) (swap id1 id2 (args CFG)).
+
+Instance swap_of_cfg : Swap cfg := swap_cfg.
+
+Instance swap_of_mcfg : Swap mcfg := swap.
+
+
+Instance swap_of_addr : Swap addr := fun id1 id2 a => a.
+Instance swap_of_int1 : Swap LLVMBaseTypes.int1 := fun id1 id2 a => a.
+Instance swap_of_int32 : Swap LLVMBaseTypes.int32 := fun id1 id2 a => a.
+Instance swap_of_int64 : Swap LLVMBaseTypes.int64 := fun id1 id2 a => a.
+Instance swap_of_ll_double : Swap LLVMBaseTypes.ll_double := fun id1 id2 a => a.
+Instance swap_of_ll_float : Swap LLVMBaseTypes.ll_float := fun id1 id2 a => a.
+
+Fixpoint swap_dvalue (id1 id2:raw_id) (dv:dvalue) : dvalue :=
+  match dv with
+  | DVALUE_FunPtr fid => DVALUE_FunPtr (swap id1 id2 fid)
+  | DVALUE_Addr a => DVALUE_Addr (swap id1 id2 a)
+  | DVALUE_I1 x => DVALUE_I1 (swap id1 id2 x)
+  | DVALUE_I32 x => DVALUE_I32 (swap id1 id2 x)
+  | DVALUE_I64 x => DVALUE_I64 (swap id1 id2 x)
+  | DVALUE_Double x => DVALUE_Double (swap id1 id2 x)
+  | DVALUE_Float x => DVALUE_Float (swap id1 id2 x)
+  | DVALUE_Undef t v => DVALUE_Undef (swap id1 id2 t) (swap id1 id2 v)
+  | DVALUE_Poison => DVALUE_Poison
+  | DVALUE_None => DVALUE_None
+  | DVALUE_Struct fields => DVALUE_Struct (List.map (fun '(t,e) => (swap id1 id2 t, swap_dvalue id1 id2 e)) fields)    
+  | DVALUE_Packed_struct fields => DVALUE_Packed_struct (List.map (fun '(t,e) => (swap id1 id2 t, swap_dvalue id1 id2 e)) fields)    
+  | DVALUE_Array elts => DVALUE_Array (List.map (fun '(t,e) => (swap id1 id2 t, swap_dvalue id1 id2 e)) elts)    
+  | DVALUE_Vector elts => DVALUE_Vector (List.map (fun '(t,e) => (swap id1 id2 t, swap_dvalue id1 id2 e)) elts)    
+  end.
+  
+Instance swap_of_dvalue : Swap dvalue := swap_dvalue.
+
+Definition swap_IO {X} (id1 id2:raw_id) (x:IO X) : IO X:=
+  match x with
+  | Alloca t => Alloca (swap id1 id2 t)
+  | Load t a => Load (swap id1 id2 t) (swap id1 id2 a)
+  | Store a v => Store (swap id1 id2 a) (swap id1 id2 v)
+  | GEP  t v vs => GEP (swap id1 id2 t) (swap id1 id2 v) (swap id1 id2 vs)
+  | ItoP  t i => ItoP (swap id1 id2 t) (swap id1 id2 i)
+  | PtoI t a => PtoI (swap id1 id2 t) (swap id1 id2 a)
+  | Call t f args => Call (swap id1 id2 t) (swap id1 id2 f) (swap id1 id2 args)
+  | DeclareFun f => DeclareFun (swap id1 id2 f)
+  end.
+
+Instance swap_of_IO {X} : Swap (IO X) := swap_IO.
+
+CoFixpoint swap_Trace X `{Swap X} (id1 id2:raw_id) (t:Trace X) : Trace X :=
+  match t with
+  | Trace.Ret x => Trace.Ret (swap id1 id2 x)
+  | Trace.Vis _ e k => Trace.Vis (swap id1 id2 e) (fun y => swap_Trace X id1 id2 (k y))
+  | Trace.Tau k => Trace.Tau (swap_Trace X id1 id2 k)
+  | Trace.Err s => Trace.Err s
+  end.
+
+Instance swap_of_Trace {X} `{SX : Swap X} : Swap (Trace X) := swap_Trace X.
+
+Check ENV.fold.
+
+(* Parameter fold : forall A: Type, (key -> elt -> A -> A) -> t elt -> A -> A. *)
+Definition swap_ENV {X} `{SX : Swap X} (id1 id2:raw_id) (m:ENV.t X) : ENV.t X :=
+  ENV.fold (fun k v n => ENV.add (swap id1 id2 k) (swap id1 id2 v) n) m (ENV.empty X).
+
+Instance swap_of_ENV {X} `{SX : Swap X} : Swap (ENV.t X) := swap_ENV.
+
+
+Definition swap_frame (id1 id2:raw_id) (f:frame) : frame :=
+  match f with
+  | KRet e id q => KRet (swap id1 id2 e) (swap id1 id2 id) (swap id1 id2 q)
+  | KRet_void e q => KRet_void (swap id1 id2 e) (swap id1 id2 q)
+  end.
+
+Instance swap_of_frame : Swap frame := swap_frame.
+
+Definition swap_result (id1 id2:raw_id) (r:result) : result :=
+  match r with
+  | Done v => Done (swap id1 id2 v)
+  | Step s => Step (swap id1 id2 s)
+  end.       
+
+Instance stawp_of_result : Swap result := swap_result.
+
+
+
+
